src/opt/FulfillStep.v
@@ -33,7 +33,7 @@ Inductive fulfill_step (lc1:Local.t) (sc1:TimeMap.t) (loc:Loc.t) (from to:Time.t
     (REL_LE: View.opt_le (TView.write_released lc1.(Local.tview) sc1 loc to releasedm ord) released)
     (REL_WF: View.opt_wf released)
     (WRITABLE: TView.writable lc1.(Local.tview).(TView.cur) sc1 loc to ord)
-    (REMOVE: Memory.remove lc1.(Local.promises) loc from to val released promises2)
+    (REMOVE: Memory.remove lc1.(Local.promises) loc from to (Message.mk val released) promises2)
     (TIME: Time.lt from to):
     fulfill_step lc1 sc1 loc from to val releasedm released ord
                  (Local.mk (TView.write_tview lc1.(Local.tview) sc1 loc to ord) promises2)
@@ -55,7 +55,7 @@ Proof.
   exploit Memory.remove_get0; eauto. i.
   inversion WF1. exploit PROMISES; eauto. i.
   exploit TViewFacts.write_future_fulfill; try apply x; try apply SC1; try apply WF1; eauto.
-  { eapply CLOSED1. eauto. }
+  { inv CLOSED1. exploit CLOSED; eauto. i. des. eauto. }
   i. des.
   esplits; eauto.
   - econs; eauto.
@@ -71,7 +71,7 @@ Lemma write_promise_fulfill
       (SC0: Memory.closed_timemap sc0 mem0)
       (MEM0: Memory.closed mem0):
   exists lc1,
-    <<STEP1: Local.promise_step lc0 mem0 loc from to val released lc1 mem2 kind>> /\
+    <<STEP1: Local.promise_step lc0 mem0 loc from to (Message.mk val released) lc1 mem2 kind>> /\
     <<STEP2: fulfill_step lc1 sc0 loc from to val releasedm released ord lc2 sc2>> /\
     <<REL: released = TView.write_released lc0.(Local.tview) sc0 loc to releasedm ord>> /\
     <<ORD: Ordering.le Ordering.strong_relaxed ord ->
@@ -96,7 +96,7 @@ Lemma fulfill_write
       (SC1: Memory.closed_timemap sc1 mem1)
       (MEM1: Memory.closed mem1):
   exists released' mem2',
-    <<STEP: Local.write_step lc1 sc1 mem1 loc from to val releasedm released' ord lc2 sc2 mem2' (Memory.op_kind_lower released)>> /\
+    <<STEP: Local.write_step lc1 sc1 mem1 loc from to val releasedm released' ord lc2 sc2 mem2' (Memory.op_kind_lower (Message.mk val released))>> /\
     <<REL_LE: View.opt_le released' released>> /\
     <<MEM: sim_memory mem2' mem1>>.
 Proof.
@@ -106,8 +106,11 @@ Proof.
   { apply WF1. eapply Memory.remove_get0. eauto. }
   i. des.
   exploit MemorySplit.remove_promise_remove;
-    try exact REMOVE; eauto; try apply WF1; try refl.
-  { eapply MEM1. apply WF1. eapply Memory.remove_get0. eauto. }
+    try exact REMOVE; (try instantiate (1:=Message.mk _ _)); eauto.
+  { try apply WF1; try refl. }
+  { econs. eauto. }
+  { inv MEM1. exploit CLOSED; [|i;des;eauto].
+    apply WF1. eapply Memory.remove_get0. eauto. }
   i. des.
   esplits; eauto.
   - econs; eauto.
@@ -118,7 +121,7 @@ Qed.
 
 Lemma promise_fulfill_write
       lc0 sc0 mem0 loc from to val releasedm released ord lc1 lc2 sc2 mem2 kind
-      (PROMISE: Local.promise_step lc0 mem0 loc from to val released lc1 mem2 kind)
+      (PROMISE: Local.promise_step lc0 mem0 loc from to (Message.mk val released) lc1 mem2 kind)
       (FULFILL: fulfill_step lc1 sc0 loc from to val releasedm released ord lc2 sc2)
       (REL_WF: View.opt_wf releasedm)
       (REL_CLOSED: Memory.closed_opt_view releasedm mem0)
@@ -141,8 +144,10 @@ Proof.
   { apply WF2. eapply Memory.promise_get2. eauto. }
   s. i. des.
   exploit MemorySplit.remove_promise_remove;
-    try exact REMOVE; eauto; try apply WF2; try refl. i. des.
-  esplits; eauto.
+    try exact REMOVE; (try instantiate (1:=Message.mk _ _)); eauto.
+  { apply WF2. }
+  { econs. eauto. }
+  i. des. esplits; eauto.
   - econs; eauto. econs; eauto.
     eapply MemoryMerge.promise_promise_promise; eauto.
   - eapply promise_lower_sim_memory. eauto.
@@ -150,7 +155,7 @@ Qed.
 
 Lemma promise_fulfill_write_exact
       lc0 sc0 mem0 loc from to val releasedm released ord lc1 lc2 sc2 mem2 kind
-      (PROMISE: Local.promise_step lc0 mem0 loc from to val released lc1 mem2 kind)
+      (PROMISE: Local.promise_step lc0 mem0 loc from to (Message.mk val released) lc1 mem2 kind)
       (FULFILL: fulfill_step lc1 sc0 loc from to val releasedm released ord lc2 sc2)
       (REL_WF: View.opt_wf releasedm)
       (REL_CLOSED: Memory.closed_opt_view releasedm mem0)
