src/prop/MemorySplit.v
@@ -20,15 +20,15 @@ Set Implicit Arguments.
 
 Module MemorySplit.
   Lemma remove_lower_remove
-        mem0 loc from to val released1 released2 mem2
-        (REL_LE: View.opt_le released2 released1)
-        (REL_WF1: View.opt_wf released1)
-        (REL_WF2: View.opt_wf released2)
+        mem0 loc from to msg1 msg2 mem2
+        (REL_LE: Message.le msg2 msg1)
+        (REL_WF1: View.opt_wf msg1.(Message.view))
+        (REL_WF2: View.opt_wf msg2.(Message.view))
         (TS: Time.lt from to)
-        (REMOVE: Memory.remove mem0 loc from to val released1 mem2):
+        (REMOVE: Memory.remove mem0 loc from to msg1 mem2):
     exists mem1',
-      <<LOWER: Memory.lower mem0 loc from to val released1 released2 mem1'>> /\
-      <<REMOVE: Memory.remove mem1' loc from to val released2 mem2>>.
+      <<LOWER: Memory.lower mem0 loc from to msg1 msg2 mem1'>> /\
+      <<REMOVE: Memory.remove mem1' loc from to msg2 mem2>>.
   Proof.
     exploit Memory.remove_get0; eauto. i.
     inv REMOVE. inv REMOVE0.
@@ -41,10 +41,7 @@ Module MemorySplit.
       replace (DOMap.remove to (Cell.raw (mem0 loc))) with
       (DOMap.remove to
                     (DOMap.add to
-                               (from,
-                                {|
-                                  Message.val := val;
-                                  Message.released := released2 |})
+                               (from, msg2)
                                (Cell.raw (mem0 loc)))).
       + econs. rewrite DOMap.gss. auto.
       + apply DOMap.eq_leibniz. ii.
@@ -64,33 +61,36 @@ Module MemorySplit.
         (REL_WF2: View.opt_wf released2)
         (REL_TO: Time.le (released1.(View.unwrap).(View.rlx) loc) to)
         (TS: Time.lt from to)
-        (REMOVE: Memory.remove promises0 loc from to val released1 promises2):
+        (REMOVE: Memory.remove promises0 loc from to (Message.mk val released1) promises2):
     exists promises1' mem1',
-      <<PROMISE: Memory.promise promises0 mem0 loc from to val released2 promises1' mem1' (Memory.op_kind_lower released1)>> /\
-      <<REMOVE: Memory.remove promises1' loc from to val released2 promises2>>.
+      <<PROMISE: Memory.promise promises0 mem0 loc from to (Message.mk val released2) promises1' mem1' (Memory.op_kind_lower (Message.mk val released1))>> /\
+      <<REMOVE: Memory.remove promises1' loc from to (Message.mk val released2) promises2>>.
   Proof.
-    exploit remove_lower_remove; eauto. i. des.
+    exploit remove_lower_remove; eauto; ss.
+    { econs. eauto. }
+    { eauto. }
+    i. des.
     exploit Memory.lower_exists_le; eauto. i. des.
     esplits; eauto.
     econs; eauto. etrans; eauto. apply View.unwrap_opt_le. ss.
   Qed.
 
   Lemma commute_remove_split_remove_remove
-        mem0 loc ts1 ts2 ts3 val2 val3 released2 released3 mem1 mem3
-        (REMOVE1: Memory.remove mem0 loc ts1 ts3 val3 released3 mem3)
-        (SPLIT1: Memory.split mem0 loc ts1 ts2 ts3 val2 val3 released2 released3 mem1):
+        mem0 loc ts1 ts2 ts3 msg2 msg3 mem1 mem3
+        (REMOVE1: Memory.remove mem0 loc ts1 ts3 msg3 mem3)
+        (SPLIT1: Memory.split mem0 loc ts1 ts2 ts3 msg2 msg3 mem1):
     exists mem2',
-      <<REMOVE3: Memory.remove mem1 loc ts1 ts2 val2 released2 mem2'>> /\
-      <<REMOVE4: Memory.remove mem2' loc ts2 ts3 val3 released3 mem3>>.
+      <<REMOVE3: Memory.remove mem1 loc ts1 ts2 msg2 mem2'>> /\
+      <<REMOVE4: Memory.remove mem2' loc ts2 ts3 msg3 mem3>>.
   Proof.
-    exploit (@Memory.remove_exists mem1 loc ts1 ts2 val2 released2); eauto.
+    exploit (@Memory.remove_exists mem1 loc ts1 ts2 msg2); eauto.
     { erewrite Memory.split_o; eauto. repeat condtac; ss.
       - guardH o. des. subst. inv SPLIT1. inv SPLIT.
         exfalso. eapply Time.lt_strorder. eauto.
       - guardH o0. des; congr.
     }
     i. des.
-    exploit (@Memory.remove_exists mem2 loc ts2 ts3 val3 released3); eauto.
+    exploit (@Memory.remove_exists mem2 loc ts2 ts3 msg3); eauto.
     { erewrite Memory.remove_o; eauto. condtac; ss.
       - des. subst. inv SPLIT1. inv SPLIT.
         exfalso. eapply Time.lt_strorder. eauto.
@@ -107,19 +107,19 @@ Module MemorySplit.
   Qed.
 
   Lemma remove_promise_promise_remove_remove
-        loc ts1 ts2 ts3 val2 released2 val3 released3
+        loc ts1 ts2 ts3 msg2 msg3
         promises0 mem0
         promises3
         (TS12: Time.lt ts1 ts2)
         (TS23: Time.lt ts2 ts3)
-        (WF2: View.opt_wf released2)
-        (TS2: Time.le (released2.(View.unwrap).(View.rlx) loc) ts2)
+        (WF2: View.opt_wf msg2.(Message.view))
+        (TS2: Time.le (msg2.(Message.view).(View.unwrap).(View.rlx) loc) ts2)
         (LE: Memory.le promises0 mem0)
-        (REMOVE: Memory.remove promises0 loc ts1 ts3 val3 released3 promises3):
+        (REMOVE: Memory.remove promises0 loc ts1 ts3 msg3 promises3):
     exists promises1 promises2 mem1,
-      <<STEP1: Memory.promise promises0 mem0 loc ts1 ts2 val2 released2 promises1 mem1 (Memory.op_kind_split ts3 val3 released3)>> /\
-      <<STEP2: Memory.remove promises1 loc ts1 ts2 val2 released2 promises2>> /\
-      <<STEP3: Memory.remove promises2 loc ts2 ts3 val3 released3 promises3>>.
+      <<STEP1: Memory.promise promises0 mem0 loc ts1 ts2 msg2 promises1 mem1 (Memory.op_kind_split ts3 msg3)>> /\
+      <<STEP2: Memory.remove promises1 loc ts1 ts2 msg2 promises2>> /\
+      <<STEP3: Memory.remove promises2 loc ts2 ts3 msg3 promises3>>.
   Proof.
     exploit Memory.remove_get0; eauto. i.
     exploit Memory.split_exists; eauto. i. des.
@@ -130,14 +130,14 @@ Module MemorySplit.
   Qed.
 
   Lemma commute_add_split_add_add
-        mem0 loc ts1 ts2 ts3 val2 val3 released2 released3 mem1 mem2
-        (ADD1: Memory.add mem0 loc ts1 ts3 val3 released3 mem1)
-        (SPLIT2: Memory.split mem1 loc ts1 ts2 ts3 val2 val3 released2 released3 mem2):
+        mem0 loc ts1 ts2 ts3 msg2 msg3 mem1 mem2
+        (ADD1: Memory.add mem0 loc ts1 ts3 msg3 mem1)
+        (SPLIT2: Memory.split mem1 loc ts1 ts2 ts3 msg2 msg3 mem2):
     exists mem1',
-      <<ADD1: Memory.add mem0 loc ts1 ts2 val2 released2 mem1'>> /\
-      <<ADD2: Memory.add mem1' loc ts2 ts3 val3 released3 mem2>>.
+      <<ADD1: Memory.add mem0 loc ts1 ts2 msg2 mem1'>> /\
+      <<ADD2: Memory.add mem1' loc ts2 ts3 msg3 mem2>>.
   Proof.
-    exploit (@Memory.add_exists mem0 loc ts1 ts2 val2 released2); eauto.
+    exploit (@Memory.add_exists mem0 loc ts1 ts2 msg2); eauto.
     { i. inv ADD1. inv ADD. hexploit DISJOINT; eauto. i.
       eapply Interval.le_disjoint; eauto. econs; [refl|].
       inv SPLIT2. inv SPLIT. left. auto.
@@ -145,7 +145,7 @@ Module MemorySplit.
     { inv SPLIT2. inv SPLIT. auto. }
     { inv SPLIT2. inv SPLIT. auto. }
     i. des.
-    exploit (@Memory.add_exists mem3 loc ts2 ts3 val3 released3); eauto.
+    exploit (@Memory.add_exists mem3 loc ts2 ts3 msg3); eauto.
     { i. revert GET2. erewrite Memory.add_o; eauto. condtac; ss.
       - des. subst. i. inv GET2.
         symmetry. apply Interval.disjoint_imm.
@@ -165,14 +165,14 @@ Module MemorySplit.
   Qed.
 
   Lemma commute_promise_add_promise_split_promise_add_promise_add
-        promises0 mem0 loc ts1 ts2 ts3 val2 val3 released2 released3
+        promises0 mem0 loc ts1 ts2 ts3 msg2 msg3
         promises1 mem1
         promises2 mem2
-        (ADD1: Memory.promise promises0 mem0 loc ts1 ts3 val3 released3 promises1 mem1 Memory.op_kind_add)
-        (SPLIT2: Memory.promise promises1 mem1 loc ts1 ts2 val2 released2 promises2 mem2 (Memory.op_kind_split ts3 val3 released3)):
+        (ADD1: Memory.promise promises0 mem0 loc ts1 ts3 msg3 promises1 mem1 Memory.op_kind_add)
+        (SPLIT2: Memory.promise promises1 mem1 loc ts1 ts2 msg2 promises2 mem2 (Memory.op_kind_split ts3 msg3)):
     exists promises1' mem1',
-      <<ADD1: Memory.promise promises0 mem0 loc ts1 ts2 val2 released2 promises1' mem1' Memory.op_kind_add>> /\
-      <<ADD2: Memory.promise promises1' mem1' loc ts2 ts3 val3 released3 promises2 mem2 Memory.op_kind_add>>.
+      <<ADD1: Memory.promise promises0 mem0 loc ts1 ts2 msg2 promises1' mem1' Memory.op_kind_add>> /\
+      <<ADD2: Memory.promise promises1' mem1' loc ts2 ts3 msg3 promises2 mem2 Memory.op_kind_add>>.
   Proof.
     inv ADD1. inv SPLIT2.
     exploit commute_add_split_add_add; try exact PROMISES; eauto. i. des.
